Move non-generated seq decls into Core file

Source/DafnyCore/Prelude/PreludeCore.bpl
@@ -960,6 +960,70 @@ axiom (forall s: Seq, x: Box :: { MultiSet#FromSeq(s)[x] }
 
 #include "Sequences.bpl"
 
+axiom (forall v: Seq, t0: Ty :: { $Is(v, TSeq(t0)) }
+  $Is(v, TSeq(t0)) <==>
+  (forall i : int :: { Seq#Index(v, i) }
+    0 <= i && i < Seq#Length(v) ==>
+    $IsBox(Seq#Index(v, i), t0)));
+
+// Build preserves $Is
+axiom (forall s: Seq, bx: Box, t: Ty :: { $Is(Seq#Build(s,bx),TSeq(t)) }
+    $Is(s,TSeq(t)) && $IsBox(bx,t) ==> $Is(Seq#Build(s,bx),TSeq(t)));
+
+function Seq#Create(ty: Ty, heap: Heap, len: int, init: HandleType): Seq;
+axiom (forall ty: Ty, heap: Heap, len: int, init: HandleType ::
+  { Seq#Length(Seq#Create(ty, heap, len, init): Seq) }
+  $IsGoodHeap(heap) && 0 <= len ==>
+  Seq#Length(Seq#Create(ty, heap, len, init): Seq) == len);
+axiom (forall ty: Ty, heap: Heap, len: int, init: HandleType, i: int ::
+  { Seq#Index(Seq#Create(ty, heap, len, init), i) }
+  $IsGoodHeap(heap) && 0 <= i && i < len ==>
+  Seq#Index(Seq#Create(ty, heap, len, init), i) == Apply1(TInt, ty, heap, init, $Box(i)));
+
+function Seq#FromArray(h: Heap, a: ref): Seq;
+axiom (forall h: Heap, a: ref ::
+  { Seq#Length(Seq#FromArray(h,a)) }
+  Seq#Length(Seq#FromArray(h, a)) == _System.array.Length(a));
+axiom (forall h: Heap, a: ref ::
+  { Seq#FromArray(h, a) }
+  (forall i: int ::
+    // it's important to include both triggers, so that assertions about the
+    // the relation between the array and the sequence can be proved in either
+    // direction
+    { read(h, a, IndexField(i)) }
+    { Seq#Index(Seq#FromArray(h, a): Seq, i) }
+    0 <= i &&
+    i < Seq#Length(Seq#FromArray(h, a))  // this will trigger the previous axiom to get a connection with _System.array.Length(a)
+    ==>
+    Seq#Index(Seq#FromArray(h, a), i) == read(h, a, IndexField(i))));
+axiom (forall h0, h1: Heap, a: ref ::
+  { Seq#FromArray(h1, a), $HeapSucc(h0, h1) }
+  $IsGoodHeap(h0) && $IsGoodHeap(h1) && $HeapSucc(h0, h1) && h0[a] == h1[a]
+  ==>
+  Seq#FromArray(h0, a) == Seq#FromArray(h1, a));
+axiom (forall h: Heap, i: int, v: Box, a: ref ::
+  { Seq#FromArray(update(h, a, IndexField(i), v), a) }
+    0 <= i && i < _System.array.Length(a) ==> Seq#FromArray(update(h, a, IndexField(i), v), a) == Seq#Update(Seq#FromArray(h, a), i, v) );
+
+// Extension axiom, triggers only on Takes from arrays.
+axiom (forall h: Heap, a: ref, n0, n1: int ::
+        { Seq#Take(Seq#FromArray(h, a), n0), Seq#Take(Seq#FromArray(h, a), n1) }
+        n0 + 1 == n1 && 0 <= n0 && n1 <= _System.array.Length(a) ==> Seq#Take(Seq#FromArray(h, a), n1) == Seq#Build(Seq#Take(Seq#FromArray(h, a), n0), read(h, a, IndexField(n0): Field)) );
+
+function Seq#Rank(Seq): int;
+axiom (forall s: Seq, i: int ::
+        { DtRank($Unbox(Seq#Index(s, i)): DatatypeType) }
+        0 <= i && i < Seq#Length(s) ==> DtRank($Unbox(Seq#Index(s, i)): DatatypeType) < Seq#Rank(s) );
+axiom (forall s: Seq, i: int ::
+        { Seq#Rank(Seq#Drop(s, i)) }
+        0 < i && i <= Seq#Length(s) ==> Seq#Rank(Seq#Drop(s, i)) < Seq#Rank(s) );
+axiom (forall s: Seq, i: int ::
+        { Seq#Rank(Seq#Take(s, i)) }
+        0 <= i && i < Seq#Length(s) ==> Seq#Rank(Seq#Take(s, i)) < Seq#Rank(s) );
+axiom (forall s: Seq, i: int, j: int ::
+        { Seq#Rank(Seq#Append(Seq#Take(s, i), Seq#Drop(s, j))) }
+        0 <= i && i < j && j <= Seq#Length(s) ==> Seq#Rank(Seq#Append(Seq#Take(s, i), Seq#Drop(s, j))) < Seq#Rank(s) );
+
 // ---------------------------------------------------------------
 // -- Axiomatization of Maps -------------------------------------
 // ---------------------------------------------------------------
